(a)
\textsc{Answer:}\vspace{-2mm}
\begin{answerlong}
\begin{align*}
110010_2 &= 1 \cdot 2^{5} + 1\cdot 2^{4} + 0 \cdot 2^{3} + 0\cdot 2^{2} + 1\cdot 2^{1} + 0\cdot 2^{0} \\
         &= 32 + 16 + 2 \\
         &= 50
\end{align*}
Therefore $110010_2 = 50$
\end{answerlong}

(b)
\textsc{Answer:}\vspace{-2mm}
\begin{answerlong}
\begin{align*}
110010_2 &= (1 \times 2^1 + 1 \times 2^0)(2^2)^2 + (0 \times 2^1 + 0 \times 2^0)(2^2)^1 + (1 \times 2^1 + 0 \times 2^0)(2^2)^0  \\
         &= 3 \times 4^2 + 0 \times 4^1 + 2 \times 4^0  \\
         &= 302_4
\end{align*}
Therefore $110010_{2} = 302_{4}$.
\end{answerlong}

(c)
\textsc{Answer:}\vspace{-2mm}
\begin{answerlong}
\begin{align*}
110010_2 &= (1 \times 2^2 + 1 \times 2^1 + 0\times 2^0) (2^3)^1 + (0 \times 2^2 + 1 \times 2^1 + 0 \times 2^0)(2^3)^0 \\
         &= 6 \times 8^1 + 2 \times 8^0 \\
         &= 62_8
\end{align*}
Therefore $110010_2 = 62_{8}$.
\end{answerlong}

(d)
\textsc{Answer:}\vspace{-2mm}
\begin{answerlong}
\begin{align*}
110010_2 &= (1 \times 2^2 + 1 \times 2^1) (2^4)^1 + (0\times 2^3 + 0 \times 2^2 + 1 \times 2^1 + 0 \times 2^0)(2^4)^0\\
         &= 3 \times 16^1 + 2 \times 16^0 \\
         &= 32_16
\end{align*}
Therefore $110010_2 = 32_{16}$.
\end{answerlong}
