(a)
\textsc{Answer:}\vspace{-2mm}
\begin{answerlong}
\begin{align*}
172_8 &= 1 \cdot 8^{2} + 7 \cdot 8^{1} + 2 \cdot 8^{0} \\
      &= 64 + 56 + 2 \\
      &= 122_{10}
\end{align*}
Therefore $172_{8} = 122_{10}$.
\end{answerlong}

(b)
\textsc{Answer:}\vspace{-2mm}
\begin{answerlong}
\begin{align*}
172_8 &= 1 \cdot (2^3)^{2} + 7 \cdot (2^3)^{1} + 2 \cdot (2^3)^{0} \\
      &= (1 \cdot 2^0) (2^3)^{2} + (1 \cdot 2^2 + 1 \cdot 2^1 + 1 \cdot 2^0) (2^3)^{1} + (0 \cdot 2^2 + 1 \cdot 2^1 + 0 \cdot 2^0) \cdot (2^3)^{0} \\
      &= 1111010_{2}
\end{align*}
Therefore $172_{8} = 1111010_{2}$.
\end{answerlong}

(c)
\textsc{Answer:}\vspace{-2mm}
\begin{answerlong}
\begin{longtable}{r|rrr}
  7 & 122 &   &   \\ \cline{2-4}
  7 &  17 & r & 3 \\ \cline{2-4}
  7 &   2 & r & 3 \\ \cline{2-4}
  2 &   0 & r & 2 \\ \cline{2-4}
\end{longtable}
Therefore $172_{8} = 233_{7}$
\end{answerlong}

(d)
\textsc{Answer:}\vspace{-2mm}
\begin{answerlong}
\begin{align*}
172_8 &= 1 \cdot (2^3)^{2} + 7 \cdot (2^3)^{1} + 2 \cdot (2^3)^{0} \\
      &= (1 \cdot 2^2 + 1 \cdot 2^1 + 1 \cdot 2^0) (2^4)^{1} + (1 \cdot 2^3 + 0 \cdot 2^2 + 1 \cdot 2^1 + 0 \cdot 2^0) \cdot (2^4)^{0} \\
      &= 7 \cdot 16 + 10 \cdot 16^0\\
      &= 7A_{16}
\end{align*}
Therefore $172_{8} = 7A_{16}$.
\end{answerlong}
